proof/SimMem.v
@@ -229,7 +229,7 @@ Section SimMemOhs.
 
   Require Import Program.
 
-  Definition sim_args `{SMOS: class} (midx: Midx.t) (ohs_src: Ohs) (ohs_tgt: Ohs)
+  Definition sim_args `{SMOS: class} (ohs_src: Ohs) (ohs_tgt: Ohs)
              (args_src args_tgt: Args.t) (smo0: SimMemOhs.t): Prop :=
     (<<SIMARGS: SimMem.sim_args args_src args_tgt smo0>>) /\
     (* (<<OHSRC: ohs_src midx ~= projT2 (smo0.(SimMemOhs.ohs_src) midx)>>) /\ *)
@@ -238,14 +238,14 @@ Section SimMemOhs.
     (* (<<OHSRC: nth_error ohs_src midx = (nth_error smo0.(SimMemOhs.ohs_src) midx)>>) /\ *)
     (* (<<OHTGT: nth_error ohs_tgt midx = (nth_error smo0.(SimMemOhs.ohs_tgt) midx)>>) *)
 
-    (<<OHSRC: ohs_src midx = (smo0.(SimMemOhs.ohs_src) midx)>>) /\
-    (<<OHTGT: ohs_tgt midx = (smo0.(SimMemOhs.ohs_tgt) midx)>>)
+    (* (<<OHSRC: ohs_src midx = (smo0.(SimMemOhs.ohs_src) midx)>>) /\ *)
+    (* (<<OHTGT: ohs_tgt midx = (smo0.(SimMemOhs.ohs_tgt) midx)>>) *)
 
-    (* (<<OHSRC: ohs_src = (smo0.(SimMemOhs.ohs_src))>>) /\ *)
-    (* (<<OHTGT: ohs_tgt = (smo0.(SimMemOhs.ohs_tgt))>>) *)
+    (<<OHSRC: ohs_src = (smo0.(SimMemOhs.ohs_src))>>) /\
+    (<<OHTGT: ohs_tgt = (smo0.(SimMemOhs.ohs_tgt))>>)
   .
 
-  Definition sim_retv `{SMOS: class} (midx: Midx.t) (ohs_src: Ohs) (ohs_tgt: Ohs)
+  Definition sim_retv `{SMOS: class} (ohs_src: Ohs) (ohs_tgt: Ohs)
              (retv_src retv_tgt: Retv.t) (smo0: SimMemOhs.t): Prop :=
     (<<SIMARGS: SimMem.sim_retv retv_src retv_tgt smo0>>) /\
     (* (<<OHSRC: ohs_src midx ~= projT2 (smo0.(SimMemOhs.ohs_src) midx)>>) /\ *)
@@ -254,11 +254,11 @@ Section SimMemOhs.
     (* (<<OHSRC: nth_error ohs_src midx = (nth_error smo0.(SimMemOhs.ohs_src) midx)>>) /\ *)
     (* (<<OHTGT: nth_error ohs_tgt midx = (nth_error smo0.(SimMemOhs.ohs_tgt) midx)>>) *)
 
-    (<<OHSRC: ohs_src midx = (smo0.(SimMemOhs.ohs_src) midx)>>) /\
-    (<<OHTGT: ohs_tgt midx = (smo0.(SimMemOhs.ohs_tgt) midx)>>)
+    (* (<<OHSRC: ohs_src midx = (smo0.(SimMemOhs.ohs_src) midx)>>) /\ *)
+    (* (<<OHTGT: ohs_tgt midx = (smo0.(SimMemOhs.ohs_tgt) midx)>>) *)
 
-    (* (<<OHSRC: ohs_src = (smo0.(SimMemOhs.ohs_src))>>) /\ *)
-    (* (<<OHTGT: ohs_tgt = (smo0.(SimMemOhs.ohs_tgt))>>) *)
+    (<<OHSRC: ohs_src = (smo0.(SimMemOhs.ohs_src))>>) /\
+    (<<OHTGT: ohs_tgt = (smo0.(SimMemOhs.ohs_tgt))>>)
   .
 
 End SimMemOhs.
